
\section{Quiver with relations}
Can all algebras over a field k be represented as $k\G$?\\\newline
\underline{No}: 
$\Lambda = \frac{k[x]}{\langle x^2\rangle} \ncong k\G \text{ for all quivers }\G
\text{dim}_{k}\Lambda = 2, \Lambda\text{ not semisimple}.\\\newline \text{Assume that}  \Lambda \cong k\G.\\
2= \text{dim}_kk\G \ge \text{\# vertices in } \G $

$ \G \colon \xymatrix{1& 2} \implies k\G$ is semisimple \blitza\\
$\implies \G$ has one vertex, $\xymatrix{1\ar@(ur,dr)^\alpha} $ $\implies$ $\text{dim}_kk\G = \infty$ \blitza\\
\newline But, $\G\colon \xymatrix{1 \ar@(ur,dr)^\alpha}$, $\Lambda \simeq \frac{k\G}{\langle \alpha^2\rangle} $\\
\rule{\textwidth}{1pt}\\
Let $\G=(\G_0,\G_1)$ be a quiver, k field.\\
\begin{defin}
\begin{enumerate}[(a)]
	~\\ \item A \emph{relation} $\sigma$ in the quiver $\G$ over k is a k-linear combination of paths
	\begin{center}
		$\sigma = a_1p_1 + a_2p_2+ \cdots + a_tp_t$\\
	\end{center}
	where $a_i\in k$, $e(p_i)=e(p_1)$ and $s(p_i)=s(p_1)$ for all $i$, and $l(p_i)\geq 2$ (the length of the path $p_i$ )
	\item if $\varrho = \{\sigma\}_{l \in T}$ is a set of relations in $\G$ over k, then $(\G,\varrho)$ is a \emph{quiver with relations over $k$.}  
\end{enumerate}
\end{defin}
\begin{exam}
	$\xymatrix{ & 1\ar[dl]_\alpha\ar[dr]^\beta & \\
		\G \colon 2\ar[dr]_\gamma & & 3\ar[dl]^\delta\\
		& 4 & }$\newline $k$ field, $\sigma = \gamma\alpha - \delta\beta$.\\\newline
		$ \G=\frac{k\G}{\langle\sigma\rangle}$. Let $M$ be a left $k\Lambda$-module. Any left $\Lambda$-module is a left $k\Lambda$-module, since $k\G \xrightarrow{\pi} \frac{k\G}{\large\sigma\rangle} = \Lambda$.\\
		$\implies M$ gives rise to a representation of $\G$.\\
		
	$\xymatrix{ & e_1M\ar[dl]_{f_\alpha = \alpha\cdot-}\ar[dr]^{\beta\cdot-=f_\beta} & \\
	 e_2M\ar[dr]_{f_\gamma=\gamma\cdot-} & & e_3M\ar[dl]^{\delta\cdot-=f_\delta}\\
	& 4 & }$\newline

$\sigma\in k\G, m \in M.$\\ $ \sigma\cdot m\defeq\pi(\sigma)\cdot m = 0\cdot m = 0, \forall m \in M$\\
$m=e_1m+e_2m+e_3m+e_4m$, $\sigma = e_4\sigma e_1$\\
$0 = \sigma\cdot m = (\gamma\alpha-\delta\beta)e_1m = \gamma(\alpha e_1m)-\delta(\beta e_1m) = f_\gamma f_\alpha(e_1m)-f_\sigma f_\beta(e_1m) = \underbrace{f_\gamma f_\alpha-f_\sigma f_\beta}_{f_\sigma}(e_im) \implies f_\sigma(e_1M)=0 \implies f_\sigma = 0 $.\\
Hence $\Lambda$-module $M$ corresponds to a representation of $\G$ satisfying the relation $\sigma(f_\sigma=0)$.\\
Conversely, we claim that a representation $(V,f)$ of $\G$ 	such that
\begin{center}
	$f_\sigma=f_\gamma f_\alpha-f_\sigma f_\beta=0$
\end{center} 
 gives a module over $\Lambda$.\\\newline
\textbf{Recall}: $I \subseteq R$ ideal: $\frac{R}{I}$-module $M$ is the same as an $R$-module $M$ such that $I\cdot M = (0)$.\\
\begin{center}
	$M = V(1) \oplus V(2) \oplus V(3) \oplus V(4) \leftarrow k\G$-module\\
	$e_1\cdot(v_1,v_2,v_3,v_4)=(v_1,0,0,0)$\\
	$\alpha\cdot(v_1,v_2,v_3,v_4)=(0,f_\alpha(v_1),0,0)$\\
\end{center}
~\\$\sigma\cdot(v_1,v_2,v_3,v_4) = (\gamma\alpha-\delta\beta)\cdot(v_1,v_2,v_3,v_4) = (0,0,0,f_\gamma f_\alpha(v_1)-f_\sigma f_\beta(v_1)) =  (0,0,0,(f_\gamma f_\alpha-f_\sigma f_\beta)(v_1)) = (0,0,0,0) $\\\newline
$\implies M$ is a $\Lambda$-module $(\Lambda=\frac{k\G}{\langle\sigma\rangle})$.
\end{exam}

\begin{exam}
$\G\colon \xymatrix{1 \ar@(ur,dr)^\alpha}, P=\{\alpha^2 \}$, $k$ field. $ \Lambda=\frac{k\G}{\langle\alpha^2\rangle}$. Find all induced $\Lambda$-modules.\\
$M$ left $\Lambda$-module $\leadsto 
(V,f) $ representation of $\G$ satisfying the relation $\alpha^2, $i.e.  $ f_{\alpha^2}=(f_\alpha)^2$\\  
	
	$\xymatrix{V \ar@(ur,dr)^{f_\alpha}}, (f_\alpha)^2=0$\\\newline
	$\implies$ The minimal polynomial of $f_\alpha$ is $x$ or $x^2$\\
	$\implies$ The ivariant factor of $f_\alpha$ is $x$ or $x^2$\\
	$\implies$ The matrix of $f_\alpha$ is similar to a direct sum of companion matrices of $x$ or $x^2$, $M_{(x)}=0$ and $M_{(x^2)}= \begin{pmatrix}0&0\\1&0\end{pmatrix}$\\~\\
	
Let T be the matrix of $f_\alpha$ w.r.t some basis $\beta$.\\
Then $\exists$ an invertible matrix $P$ such that\newline
	
$ T = P \underbrace{ \left(\begin{smallmatrix} r\begin{cases} \left(\begin{smallmatrix} 0 \cdots 0  \\\vdots \ddots \vdots \\0 \cdots 0 \end{smallmatrix}\right) \end{cases} & \overbrace{\text{\huge0}}^{2s}\\\text{\huge0} & 
\left(\begin{smallmatrix}  
\left( \begin{smallmatrix} 0 & 0\\ 1 & 0\\ \end{smallmatrix}\right) & & & \text{\huge0}  \\
& \begin{smallmatrix} 0 & 0\\ 1 & 0\\ \end{smallmatrix} & & \\
& &\ddots &  & \\
\text{\huge0} & & &\begin{smallmatrix} 0 & 0\\ 1 & 0\\ \end{smallmatrix} \\
\end{smallmatrix}\right) \end{smallmatrix}\right)}_{T_0}P^{-1} $ $\implies TP= PT_0$ \nolinebreak[4]\\\newline
$\xymatrix{V \ar@(ur,dr)^{T}} \iff \xymatrix{V \ar@(ur,dr)^{T_0}} \simeq (\xymatrix{k \ar@(ur,dr)^{0}})^r \oplus (\xymatrix{k^2 \ar@(ur,dr)^{\left(\begin{smallmatrix}0&0\\1&0\end{smallmatrix}\right)}})^s  $  isomorphisme of representation

\textbf{Show}: $\xymatrix{k \ar@(ur,dr)^{0}} \iff \frac{k\G}{\langle\alpha\rangle}$ and $\xymatrix{k^2 \ar@(ur,dr)^{\left(\begin{smallmatrix}0&0\\1&0\end{smallmatrix}\right)}} \iff \frac{k\G}{\langle\alpha^2\rangle} \implies \Lambda$ is of finite representation type.
\end{exam}
\subsection{Finite length}
$\Lambda$ ring, $A$ a (left) $\Lambda$-module.
\begin{defin}
	A has \emph{finite length}\index{finite length} if there exists a finite filtration.\\
	\begin{center}
			$\mathscr{F}\colon A = A_0 \supseteq A_1 \supseteq A_2 \supseteq \cdots A_{n-1} \supseteq A_{n} \supseteq A_{n+1} = (0) $\\
	\end{center}
of submodules of $A$ such that $\frac{A_i}{A_{i+1}} = 0$ or simple for i$=0,1,\cdots,n.$. 	$\mathscr{F}$ is a \emph{generalized composition series}\index{generalized composition series} of $A$, and if $\frac{A_i}{A_{i+1}} \ne 0$ for all i, then $\mathscr{F}$ is a \emph{composition series}\index{composition series}. If $S=\frac{A_i}{A_{i+1}} \ne 0$, then $S$ is called a \emph{composition factor of $A$}\index{composition factor}\\

Let $S$ be a simple $\Lambda$-module. Let
\begin{equation*}
m_s^{\mathscr{F}}(A) \defeq\{i \mid \frac{A_i}{A_{i+1}}\simeq S \}\mid
\text{ , }\notag\\
l_{\mathscr{F}} \defeq \sum_{\mathclap{\substack{\small[S]
      \text{isomorphism} \\ \small\text{classes of
        simples}}}}m_s^{\mathscr{F}}(A)\notag\\
\intertext{ and }\notag\\
l(A) \defeq \min_{\mathclap{\substack{\mathscr{F} \text{generalized} \\ \text{composition series}}}} l_{\mathscr{F}}(A)\notag
\end{equation*}
\end{defin}

\begin{exam}
	\begin{enumerate}[(1)]
		\item $\Lambda$ ring, $S$ simple $\Lambda$-module.\\
		Composition series: $S \supseteq (0)$\\
		composition factors: $\{S\}$\\
		$\implies m_T(S) = \left\{\!\begin{aligned}
			&1 &\text{if } T \simeq S\\[1ex]
			&0 &\text{otherwise}\\[1ex]
		\end{aligned}\right\}\implies l(S)=1$
		\item $\Lambda = k[x], f(x)$ irredicible\\
		$S_f=\frac{k[x]}{\langle f(x) \rangle}$ - simple $\Lambda$- module.\\
		$\implies l(S_f)=1$, while $\dim_kS_f = \deg f(x)$ \\
		\item $\G\colon  \xymatrix{1\ar[r]^\alpha & 2\ar[r]^\beta & }, k \text{ field } , \Lambda=k\G$\\
		$
		\xymatrix
		{
			& k\ar[d]^1 & 0 \ar[l]^0\ar[d]^0  & 0\ar[l]^0\ar[d]^0 & 0\ar[l]^0\ar[d]^0 \\
		\mathscr{F}\colon	&k \ar[d]^1  & k\ar[l]^1\ar[d]^1 & 0\ar[l]^0\ar[d]^0 & 0\ar[l]^0\ar[d]^0 \\
			&k \ar@{}[d]|-*[@]{=}& k\ar@{}[d]|-*[@]{=} & k\ar@{}[d]|-*[@]{=} & 0\ar@{}[d]|-*[@]{=} \\\
			&V_o\ar@{<~>}[d] & V_1\ar@{<~>}[d] & V_2\ar@{<~>}[d] & V_3\ar@{<~>}[d]\\
			M \ar@{}[r]|-*[@]{=} & M_0 \ar@{}[r]|-*[@]{\supseteq}  &  M_1 \ar@{}[r]|-*[@]{\supseteq} & M_2 \ar@{}[r]|-*[@]{\supseteq} & M_3 = (0) \\
		}$\\~\\
	
	$\xymatrix
	{
		& k\ar[d] & \\
		\frac{V_0}{V_1} \ar@{}[r]|-*[@]{\simeq}	& 0\ar[d]\ar@{<~>}[r] & S_1 , \\
		& 0 & \\
	}$
$\xymatrix
{
	& k\ar[d] & \\
	\frac{V_1}{V_2} \ar@{}[r]|-*[@]{\simeq}	& 0\ar[d]\ar@{<~>}[r] & S_2 , \\
	& 0 & \\
}$
$\xymatrix
{
	& k\ar[d] & \\
	\frac{V_2}{V_3} \ar@{}[r]|-*[@]{\simeq}	& 0\ar[d]\ar@{<~>}[r] & S_3 \\
	& 0 & \\
}$\\
$\implies l_{\mathscr{F}}(M)=3$\\~\\

\item $\G \xymatrix{ & 1\ar[dr]^{\beta} \ar[dl]_{\alpha} & \\ 2 & & 3  } , k$ field, $ M = k\G e_1 \iff \xymatrix{ & k\ar[dr]^{1} \ar[dl]_{1} & \\ k & & k }\\$
need more	!!!!!!!!!!!!!!!!!!!!!
\end{enumerate}
\end{exam}

\begin{note}
	\begin{enumerate}[(1)]
		\item Composition serice are not unique!
		\item $l_{\mathscr{F}}(M) = l_{\mathscr{G}}(M)$
		\item The set of composition factors is the same for $\mathscr{F}$ and $\mathscr{G}$
	\end{enumerate}
\end{note}
\rule{\textwidth}{1pt}\\
The proof of Jordan-HÃ¸lder theorem goes bu induction on length and using short exact sequences.
\begin{defin}
	$\xymatrix{0 \ar[r] & A\ar[r]^f & B\ar[r]^g & C \ar[r] & 0}$ is a \emph{text}((short) exact sequence)\index{exact sequence} of (left) $\Lambda$-module if
	\begin{enumerate}[(i)]
		\item $f$ is injective (1-1)
		\item $g$ is surjective (onto)
		\item Im(f) = ker(g)
	\end{enumerate}
\end{defin} 
\begin{note}
	\begin{enumerate}[(1)]
		\item $A \supseteq B \Lambda$-modules, submodule then\\
		\begin{center}
			$\xymatrix{0 \ar[r] & A\ar[r]^f & B\ar[r]^g & C \ar[r] & 0}$
		\end{center}
	is an exact sequence
	\item If $\xymatrix{0 \ar[r] & A\ar[r]^f & B\ar[r]^g & C \ar[r] & 0}$ is an exact sequence, then
	\begin{enumerate}[(a)]
		\item $C = \text{Im}(g) \simeq \frac{B}{\text{Ker(g)}} \simeq \frac{B}{\text{Im(f)}}, \text{Im}(f)\simeq A. $
		\item $B = (0) \implies A = (0) \text{ and } C=(0). $ 
	\end{enumerate}
	\end{enumerate}
\end{note}

\begin{exam}
	\begin{enumerate}[(1)]
		\item  $\xymatrix{0 \ar[r] & \mathbb{Z}\ar[r]^{-\cdot n} & \mathbb{Z}\ar[r] & \frac{\mathbb{Z}}{n\mathbb{Z}} \ar[r] & 0}$ exact
		\item $M, N$ $\Lambda$-modules.
		$\xymatrix
		{
			0\ar[r] & M\ar[r]^{\left(\begin{smallmatrix} 1 \\ 0 \end{smallmatrix}\right)} & M\oplus N\ar[r]^{\left(\begin{smallmatrix} 1 & 0 \end{smallmatrix}\right)} & N & O \\
			  & m \ar@{|->}[r]& (m,0) \\
			  &   & (m,n) \ar@{|->}[r]    & n\\
		}$ exact
	\item $\Lambda = \frac{k\G}{\langle p \rangle}$, $\xymatrix{0 \ar[r] & A\ar[r]^f & B\ar[r]^g & C \ar[r] & 0}$ exact sequence of $\Lambda$-modules.
	$\xymatrix
	{
		 & V_A(i)\ar@{}[d]|-*[@]{=} \ar[r]^{f\vert_{V_A(i)}} & V_B(i)\ar@{}[d]|-*[@]{=} \ar[r]& V_C(i)\ar@{}[d]|-*[@]{=} & \\
		0\ar[r]& e_iA \ar[r]^{f\vert_{e_iA}}  & e_iB  \ar[r]^{g\vert_{e_iB}}  & e_iC \ar[r]  & 0\\
	}$ exact sequence for all i\\
Hence, 	$\xymatrix{0 \ar[r] & (V',f')\ar[r]^g & (V,f)\ar[r]^h & (V'',f'') \ar[r] & 0}$ is an exact sequence of representation if $\xymatrix{0 \ar[r] & V'(i)\ar[r]^{g(i)} & V(i)\ar[r]^{h(i)} & V''(i) \ar[r] & 0}$ is exact for all i $\in\G_0$
	
	\end{enumerate}
\end{exam}
\rule{\textwidth}{1pt}\\
\begin{exer}
		$f\colon\xymatrix{A\ar[r] & B}$ and $g\colon\xymatrix{B\ar[r] & C}$, $\Lambda$-homomorphisme, $B' \subseteq B$ submodule.
		\begin{enumerate}[(1)]
			\item $f^{-1}(B')= \{ a\in A\mid f(a)\in B'\}\subseteq A$ submodule
			\item $g(B')= \{ g(b')\mid b'\in B'\}\subseteq C$ submodule
		\end{enumerate}
\end{exer}
\rule{\textwidth}{1pt}\\
Let $\xymatrix{0 \ar[r] & A\ar[r]^f & B\ar[r]^g & C \ar[r] & 0}$ be an exact sequence and let $\mathscr{F}$ be a generalized composition series of B.\\
$\xymatrix
{
	0\ar[r] & A\ar[r]^f & B\ar[r]^g\ar & C\ar[r] & 0\\
			& A_o=f^{-1}(B_0)\ar@{}[u]|-*[@]{=}	  & B_0	\ar@{}[u]|-*[@]{=}				& g(B_0)= C_0\ar@{}[u]|-*[@]{=} \\
			& A_1=f^{-1}(B_1)\ar@{}[u]|-*[@]{\subseteq} & B_1\ar@{}[u]|-*[@]{\subseteq}& g(B_1)= C_1\ar@{}[u]|-*[@]{\subseteq} \\
			& A_2=f^{-1}(B_2)\ar@{}[u]|-*[@]{\subseteq} & B_2\ar@{}[u]|-*[@]{\subseteq}& g(B_2)= C_2\ar@{}[u]|-*[@]{\subseteq} \\
			& \vdots\ar@{}[u]|-*[@]{\subseteq} & \vdots\ar@{}[u]|-*[@]{\subseteq}& \vdots\ar@{}[u]|-*[@]{\subseteq} \\
			& A_n=f^{-1}(B_n)=(0)\ar@{}[u]|-*[@]{\subseteq} & B_n=(0)\ar@{}[u]|-*[@]{\subseteq}& g(B_n)= C_n=(0)\ar@{}[u]|-*[@]{\subseteq} \\
			& \mathscr{F}'\ar@{}[u]|-*[@]{\colon} & \mathscr{F}\ar@{}[u]|-*[@]{\colon}& \mathscr{F}''\ar@{}[u]|-*[@]{\colon} \\
}$
\begin{prop}
	\begin{enumerate}[(a)]
		\item $\mathscr{F}'$ is generalized composition series of $A$.\\
		$\mathscr{F}''$ is generalized composition series of $C$.\\
		\item $m^{\mathscr{F}}_S(B)=m^{\mathscr{F}'}_S(A) + m^{\mathscr{F}''}_S(C) \forall S$ simple
	\end{enumerate}
\end{prop}