\subsection{Modules and representations}

$\Gamma = (\Gamma_0,\Gamma_1)$ - quiver, $k$ field.

$M$ left $k\Gamma$-module $\leadsto\begin{cases}
(V,f) \text{\ representation of $\Gamma$}\\
V(i) = e_iM\\
\text{for\ } \alpha\colon i\to j \in \Gamma_1, \text{\ we have\ }  f_\alpha\colon
V(i)=e_iM\extto{\alpha\cdot -} e_jM = V(j)\\
f_\alpha(e_im) = \alpha e_im
\end{cases}$

$(V,f)$ representaion of $\Gamma\leadsto \begin{cases}
M = \oplus_{i\in\Gamma_0} V(i)\\
m = (v_1,v_2,\ldots, v_n) \in M\\
e_im \extto{\text{def}}{=} (0,\ldots,0,v_i,0,\ldots,0)\\
\text{for $\alpha\colon i\to j$ in $\Gamma_1$, remember $\alpha =
  e_j\alpha e_i$}\\
\alpha m \extto{\text{def}}{=} (0,\ldots,0,f_\alpha(v_i),0,\ldots,0)
\text{\ with $f_\alpha(v_i)$ in the $j$-th coordinate}
\end{cases}$

\begin{exam}
$\Gamma\colon \xymatrix{1\ar[r]^\alpha & 2}$, $k$ field.

$(V,f)\colon \xymatrix{k\ar[r]^1 & k} \leadsto M = k\oplus k = k^2$

\begin{align}
e_1\cdot (a,b) & = (a, 0)\notag\\
e_2\cdot (a,b) & = (0,b)\notag\\
\alpha\cdot(a,b) & = (0,a)\notag
\end{align}
Note: $k\Gamma e_1 = k\{ e_1,\alpha\}$.  Define $\varphi\colon M\to
k\Gamma e_1$ by letting 
\[\varphi(1,0) = e_1 \text{\ and\ } \varphi(0,1) = \alpha.\]

Have: 
\begin{align}
\alpha \varphi(a,b)  & = \alpha(ae_1 + b\alpha) =
a\underbrace{\alpha e_1}_{=\alpha} +
                       b\underbrace{\alpha^2}_{=0}\notag\\
& = a\alpha\notag\\
& = \varphi(0,a) = \varphi(\alpha(a,b))\notag
\end{align} 
Similarly, $e_i\varphi(a,b) = \varphi(e_i(a,b))$. This implies that
$\varphi$ is a $k\Gamma$-homomorphism.\medskip 

$\left.\begin{matrix}
\Ker \varphi = (0)\\
\Im\varphi = k\Gamma e_1
\end{matrix}\right\} \Rightarrow M\simeq k\Gamma e_1 \text{\ as a left $k\Gamma$-module}.$



\end{exam}
